\subsection*{a}
\begin{align*}
    &f(n)= 2n+300\\
    &g(n) =100 n + 2 
\end{align*}
Using rules of limits of equations:
\begin{align*}
    \lim_{n \to \infty}\frac{f(n)}{g(n)} &\equiv \lim_{n \to \infty}\frac{2n + 300}{100n + 2}\\
    &\equiv \lim_{n \to \infty} \frac{2n}{100n}\\
    &=  \frac{2}{100} =\frac{1}{50}
\end{align*}
Since $\lim_{n \to \infty} \frac{f(n)}{g(n)} = C $ where $C \in \R$, $f(n) \in \Theta(g(n))$

\subsection*{b}
\begin{align*}
    f(n) &= n^{\frac{3}{4}}\\
    g(n) &= n^{\frac{2}{3}}
\end{align*}
\begin{align*}
    \lim_{n \to \infty} \frac{f(n)}{g(n)} &= \lim_{n \to \infty} \frac{n^{\frac{3}{4}}}{n^{\frac{2}{3}}}\\
    &= \lim_{n \to \infty} n^{\frac{3}{4} - \frac{2}{3}}\\
    &= \lim_{n \to \infty} n^{\frac{1}{12}} = 0
\end{align*}
Since $\lim_{n \to \infty} \frac{f(n)}{g(n)} = 0 $, $f(n) \in O(g(n))$.

\subsection*{c}
\begin{align*}
    f(n) &= 10n^2 + (log_2(n))^3\\
    g(n) &= n + log_2(n)
\end{align*}
\begin{align*}
    \lim_{n \to \infty} \frac{f(n)}{g(n)} &= \lim_{n \to \infty} \frac{10n^2 + (log_2(n))^3}{n + log_2(n)}\\
    &= \lim_{n \to \infty} \frac{10n^2}{n}\\
    &= \lim_{n \to \infty} 10n = \infty
\end{align*}
Since $\lim_{n \to \infty} \frac{f(n)}{g(n)} = \infty$, $f(n) \in \Omega(g(n))$

\subsection*{d}
\begin{align*}
    f(n) &= 37 n \log(10^6n)\\
    g(n) &= n log(n)
\end{align*}
\begin{align*}
    \lim_{n \to \infty} \frac{f(n)}{g(n)} &= \frac{37 n \log(10^6 n)}{n \log (n)}\\
    &= \lim_{n \to \infty} \frac{37(\log(10^6) + \log(n))}{\log(n)}\\
    &= \lim_{n \to \infty} \frac{37 * \log(10^6)}{\log(n)} + 1\\
    &= 1
\end{align*}
Since $\because \exists C \in \R ^+ S.T. \lim_{n \to \infty} \frac{f(n)}{g(n)} = C$, $f(n) \in \Theta(g(n))$

\subsection*{e}
\begin{align*}
    f(n) &= n^2 \log n\\
    g(n) &= n^{2.0001}(log(n)^2
\end{align*}{}
\begin{align*}
    \lim_{n \to \infty} \frac{f(n)}{g(n)} &= \lim _{n \to \infty} \frac{n^2 \log n}{n^{2.0001} (\log (n)) ^ 2 }\\
    &= \lim_{n \to \infty}( \frac{n^2}{n^{2.0001}} \frac{\log(n)}{\log(n) * \log(n)})\\
    &= \lim_{n \to \infty} \frac{1}{n^{0.0001}log(n)}\\
    &= 0\\
    &\implies f(n) \in O(g(n))
\end{align*}

\subsection*{f}
\begin{align*}
    f(n) &= (\log(n))^2\\
    g(n) &= \frac{n}{\log(n)}
\end{align*}
\begin{align*}
    \lim_{n \to \infty}\frac{f(n)}{g(n)} &= \lim_{n \to \infty}(\frac{\log(n)* \log(n)}{\frac{n}{\log(n)}})\\
    &= \lim_{n \to \infty}(\frac{(\log(n))^3}{n})\\
    &= \lim_{n \to \infty} \frac{1}{n}\\
    &= 0\\
    &\implies f(n) \in O(g(n))
\end{align*}

\subsection*{g}
\begin{align*}
    f(n) &= \frac{n}{\log(n)}\\
    g(n) &= (\log n)^{\log(n)}
\end{align*}

\begin{align*}
    \lim_{n \to \infty} \frac{f(n)}{g(n)} &= \frac{\frac{n}{\log(n)}}{(\log(n))^{\log(n)}}\\
    &= \lim_{n \to \infty} \frac{n (\log(n))^{-1}}{(\log(n)^{\log(n)}}\\
    &= \lim_{n \to \infty} (n (\log(n))^{\log(n)-1})\\
    &= \lim_{n \to \infty} (n (\log(n))^{\log(n) - \log_2(2)}\\
    &= \lim_{n \to \infty} n (\log(n))^{\log(n/2)}\\
    &= \infty\\
    &\implies f(n) \in \Omega(g(n)) \And f(n) \not\in(O(g(n))
\end{align*}

\subsection*{h}
\begin{align*}
    f(n) = (\log(n))^3\\
    g(n) = \sqrt[3]{n}
\end{align*}
\begin{align*}
    \lim_{n \to \infty}\frac{f(n)}{g(n)} &= \lim_{n \to \infty}\frac{(\log(n))^3}{\sqrt[3]{n}}\\
    &= \lim_{n \to \infty} \frac{3(\log(n))^2 \frac{1}{n \ln 2}}{\frac{1}{3} n ^ {-\frac{2}{3}}} \text{ (By L'Hopital's Law)}\\
    &= \lim_{n \to \infty}\frac{3n^{\frac{2}{3}}*3*(\log(n))^2 }{n \ln(2)}\\
    &= \lim_{n \to \infty}\frac{9 (\sqrt[3]{n}\log(n))^2}{n \ln(2)}\\
    &= \lim_{n \to \infty}\frac{9 * 2 (\sqrt[3]{n}log(n))(\sqrt[3]{n}\frac{1}{n \ln(2)} + \frac{1}{3}log(n)n^{-\frac{2}{3}})}{\ln(2)} \text{ (By L'Hopital's Law)}\\
    &= 18 \lim_{n \to \infty} \frac{\frac{n^{\frac{2}{3}}log(n)}{n \ln 2} + n^{-\frac{1}{3}} (\log(n))^2}{\ln(2)}\\
    &= 0\\
    &\implies f(n) \in O(g(n))
\end{align*}
\subsection*{i}
\begin{align*}
    f(n) &= 3^{\log_2(n)}\\
    g(n) &= n^{\log_2(3)}
\end{align*}
\begin{align*}
    \lim_{n \to \infty} \frac{f(n)}{g(n)} &= \lim_{n \to \infty} \frac{3^{\log_2(n)}}{n^{\log_2(3)}}\\
    &= \frac{3^{\frac{\log_3(n)}{\log_3(2)}}}{n^{\log_2(3)}}\\
    &= \frac{3^{\log_3(n) (\frac{1}{\log_3(2)})}}{n^{\log_2(3)}}\\
    &= \lim_{n \to \infty}\frac{n^{\log_3(2)}}{n^{\log_2(3)}}\\
    &= \lim_{n \to \infty} n^{\log_3(2) - \log_2(3)}\\
    &\because \log_3(2) < 1 \And \log_2(3) > 1 \log_3(2) - \log_2(3) < 0\\
    &\therefore \exists C \in \R^+: n^{\log_3(2) - \log_2(3)} =  n^{-C}\\
    &\And \lim_{n \to \infty} n^{-C} = 0\\
    &\implies f(n) \in O(g(n)) \because \lim_{n \to \infty} \frac{f(n)}{g(n)} = 0
\end{align*}

\subsection*{j}
\begin{align*}
    f(n) &= 3^n\\
    g(n) ^= n^42^n
\end{align*}
\begin{align*}
    \lim_{n \to \infty} \frac{f(n)}{g(n)} &= \lim_{n \to \infty}\frac{3^n}{n^42^n}\\
    &\lim_{n \to \infty} \frac{1.5^n}{n^4}\\
    &= \infty\\
    &\implies f(n) \in \Omega(g(n))
\end{align*}

\subsection*{k}
\begin{align*}
    f(n) &= n!\\
    g(n) &= 2^n
\end{align*}

\begin{align*}
    \lim_{n \to \infty}\frac{f(n)}{g(n)} &= \lim_{n \to \infty}(\frac{n!}{2^n}\\
    &= \infty\\
    \implies f(n) \in \Omega(g(n))
\end{align*}

\subsection*{l}
\begin{align*}
    f(n) &\triangleq 2^{(\log(n))^2}\\
    g(n) &\triangleq (\log(n))^{(\log(n))}
\end{align*}

\begin{align*}
    \lim_{n \to \infty} \frac{f(n)}{g(n)} &= \lim_{n \to \infty} \frac{2^{(\log(n))^{2}}}{(log(n))^{\log(n)}}\\
    &= \lim_{n \to \infty} \frac{2^{(\log(n)\log(n)}}{(\log(n))^{\log(n)}}\\
    &= \lim_{n \to \infty} \frac{(2^{\log(n)})^{(\log(n)}}{(\log(n))^{(\log(n)}}\\
    &\because \forall n > 2 \log(n) > 1, 2^{\log(n)} > \log(n) \text{ for large n}\\
    &\implies \lim_{n \to \infty} 2^{\log(n)}^{\log(n)} > \lim_{n \to \infty} (\log(n))^{(\log(n)}\\
    &\because \lim_{n \to \infty} \log(n)^{\log(n)} = \infty, \lim_{n \to \infty} \frac{(2^{\log(n)})^{\log(n)})}{(\log(n))^{\log(n)}} = \infty\\
    &\implies f(n) \in \Omega(g(n))
\end{align*}
